

## MATH-4007 Calculus 2 class 14

B13902126 胡允升

**Description.** Find the following the indefinite integral

$$\int x(\ln x)^2 \, dx$$

**Correct Ans.**

$$\frac{x^2(\ln x)^2}{2} - x^2 \ln x + \frac{x^2}{4} + C$$

**Reason.** See the following steps:

1° let  $u = \ln x$  ( $dx = \frac{1}{x} du$ ), then do the substitution to get

$$\int x(\ln x)^2 \, dx = \int e^u u^2 (x \, du) = \int u^2 e^{2u} \, du$$

2° Use integration by parts twice:

	D	I
+	$u^2$	$e^{2u}$
-	$2u$	$\frac{1}{2}e^{2u}$
+	$2$	$\frac{1}{4}e^{2u}$

we have

$$\begin{aligned} \int u^2 e^{2u} \, du &= \frac{1}{2} u^2 e^{2u} - \frac{1}{2} u e^{2u} + \frac{1}{2} \int e^{2u} \, du \\ &= \frac{1}{2} u^2 e^{2u} - \frac{1}{2} u e^{2u} + \frac{1}{4} e^{2u} + C \\ &= \frac{x^2(\ln x)^2}{2} - x^2 \ln x + \frac{x^2}{4} + C \end{aligned}$$

**Description.** Find the following the indefinite integral

$$\int \frac{5}{[(ax)^2 - b^2]^{3/2}} dx$$

**Correct Ans.**

$$-\frac{5}{ab\sqrt{b^2 - a^2x^2}} + C$$

**Reason.** We have to convert it into a standard form

$$\sec^2 \theta = 1 + \tan^2 \theta$$

So we let  $x = \frac{b}{a} \sec \theta$  and we get

$$\begin{aligned} \int \frac{5}{[(ax)^2 + b^2]^{3/2}} dx &= \int \frac{5}{[a^2(\frac{b}{a} \sec \theta)^2 + b^2]^{3/2}} \cdot \frac{b}{a} \sec \theta \tan \theta \, d\theta \\ &= \int \frac{5}{[b^2 \sec^2 \theta + b^2]^{3/2}} \cdot \frac{b}{a} \sec \theta \tan \theta \, d\theta \\ &= \int \frac{5}{b^3(\sec^2 \theta)^{3/2}} \cdot \frac{b}{a} \sec \theta \tan \theta \, d\theta \\ &= \frac{5}{ab^2} \int \frac{\cos \theta}{\sin^2 \theta} \, d\theta \end{aligned}$$

then, let  $u = \sin \theta$  ( $d\theta = \frac{1}{\cos \theta} du$ ), we have

$$\begin{aligned} \frac{5}{ab^2} \int \frac{\cos \theta}{\sin^2 \theta} \, d\theta &= \frac{5}{ab^2} \int \frac{\cos \theta}{u^2} \cdot \frac{1}{\cos \theta} du \\ &= \frac{5}{ab^2} \int u^{-2} du \\ &= \frac{5}{ab^2} \cdot (-u^{-1}) + C \\ &= -\frac{5}{ab^2 \sin \theta} + C \end{aligned}$$

Finally, we have to convert back to  $x$ :

$$\sin \theta = \sqrt{1 - \cos^2 \theta} = \sqrt{1 - \left(\frac{ax}{b}\right)^2} = \frac{\sqrt{b^2 - a^2x^2}}{b}$$

Thus, the final answer is

$$-\frac{5}{ab^2} \cdot \frac{b}{\sqrt{b^2 - a^2x^2}} + C = -\frac{5}{ab\sqrt{b^2 - a^2x^2}} + C$$

**Description.** Find the following the indefinite integral

$$\int -6 \ln(x^2 - 1) \, dx$$

**Correct Ans.**

?

**Reason.** Do the factorization first:

$$\int -6 \ln(x^2 - 1) \, dx = \int -6 \ln(x - 1) \, dx + \int -6 \ln(x + 1) \, dx$$

Then, we can do the integration by parts for each part:

1° for  $\int -6 \ln(x - 1) \, dx$ :

	D	I
+	$-6 \ln(x - 1)$	1
-	$-\frac{6}{x-1}$	$x$

we have

$$\begin{aligned} \int -6 \ln(x - 1) \, dx &= -6x \ln(x - 1) + 6 \int \frac{x}{x - 1} \, dx \\ &= -6x \ln(x - 1) + 6 \int \left(1 + \frac{1}{x - 1}\right) \, dx \\ &= -6x \ln(x - 1) + 6x + 6 \ln|x - 1| + C \end{aligned}$$

2° for  $\int -6 \ln(x + 1) \, dx$ :

	D	I
+	$-6 \ln(x + 1)$	1
-	$-\frac{6}{x+1}$	$x$

we have

$$\begin{aligned} \int -6 \ln(x + 1) \, dx &= -6x \ln(x + 1) + 6 \int \frac{x}{x + 1} \, dx \\ &= -6x \ln(x + 1) + 6 \int \left(1 - \frac{1}{x + 1}\right) \, dx \\ &= -6x \ln(x + 1) + 6x - 6 \ln|x + 1| + C \end{aligned}$$

**Description.** Find the following the indefinite integral

$$\int x^2 \arctan(5x) \, dx$$

**Correct Ans.**

$$\frac{x^3}{3} \arctan(5x) - \frac{5}{3} \cdot \frac{1}{1250} (1 + 25x^2 - \ln |1 + 25x^2|) + C$$

**Reason.** Doing the integration by parts follow the LIATE rule:

	D	I
+	$\arctan(5x)$	$x^2$
-	$\frac{5}{1+25x^2}$	$\frac{x^3}{3}$

We get

$$\int x^2 \arctan(5x) \, dx = \frac{x^3}{3} \arctan(5x) - \frac{5}{3} \int \frac{x^3}{1 + 25x^2} \, dx$$

Use substitution  $u = 1 + 25x^2$  to solve the remaining integral.

$$\begin{aligned} \int \frac{x^3}{1 + 25x^2} \, dx &= \int \frac{x^3}{u} \cdot \frac{du}{50x} = \frac{1}{50} \int \frac{(u-1)/25}{u} du \\ &= \frac{1}{1250} (u - \ln |u|) + C \end{aligned}$$

Thus, the final answer is

$$\frac{x^3}{3} \arctan(5x) - \frac{5}{3} \cdot \frac{1}{1250} (1 + 25x^2 - \ln |1 + 25x^2|) + C$$

**Description.** Let  $I_n = \int \sec^n(x) \, dx$ . Prove that

$$I_n = \frac{1}{n-1} \tan x \sec^{n-2}(x) + \frac{n-2}{n-1} I_{n-2}$$

**Reason.** First imply the integration by parts:

	D	I
+	$\sec^{n-2}(x)$	$\sec x \tan x$
-	$(n-2) \sec^{n-3}(x) \sec x \tan x$	$\sec x$

Then we get

$$\begin{aligned}
 I_n &= \int \sec^{n-2}(x) \sec^2(x) \, dx \\
 &= \tan(x) \sec^{n-2}(x) - (n-2) \int \sec^{n-2}(x) \tan^2(x) \, dx \\
 &= \tan(x) \sec^{n-2}(x) - (n-2) \int \sec^{n-2}(x) (\sec^2 x - 1) \, dx \\
 &= \tan(x) \sec^{n-2}(x) - (n-2) \underbrace{\int \sec^n(x) \, dx}_{I_n} + (n-2) \underbrace{\int \sec^{n-2}(x) \, dx}_{I_{n-2}} \\
 &= \tan(x) \sec^{n-2}(x) - (n-2) I_n + (n-2) I_{n-2}
 \end{aligned}$$

Rearranging the equation, we have

$$I_n = \frac{1}{n-1} \tan x \sec^{n-2}(x) + \frac{n-2}{n-1} I_{n-2}$$